Add preliminary version of Assigned
Make small adjustments in Coloring and Instructions.

Coloring.v
@@ -5,7 +5,7 @@ Module Coloring (Owner : DecidableType) (Map : WSfun Owner).
   Module Import Facts := WFacts_fun Owner Map.
 
   Definition t : Type :=
-      nat * Map.t nat.
+    nat * Map.t nat.
 
   Definition colors (self : t) : nat :=
     fst self.
@@ -17,7 +17,7 @@ Module Coloring (Owner : DecidableType) (Map : WSfun Owner).
   Definition Contains (self : t) (owner : Owner.t) : Prop :=
     Map.In owner (labeling self).
 
-    Program Definition find
+  Program Definition find
     (self : t)
     (owner : Owner.t | Contains self owner) :
     {color : nat | MapsTo self owner color} :=
@@ -33,72 +33,97 @@ Module Coloring (Owner : DecidableType) (Map : WSfun Owner).
       now apply not_find_in_iff in H.
     Qed.
 
+  Definition find'
+    (self : t)
+    (owner : Owner.t) :
+    option nat :=
+      Map.find owner (labeling self).
+
   Definition Ok (coloring : nat * Map.t nat) :=
     forall color : nat,
       color < colors coloring <->
       (exists owner : Owner.t, MapsTo coloring owner color).
 
-  Program Definition empty : {self' : t | Ok self'} :=
+  Definition empty :
+    t :=
     (0, Map.empty nat).
-  Next Obligation.
-    intros color.
-    split.
-      intros color_lt_colors.
-      contradict color_lt_colors; auto with arith.
-    intros [owner owner_to_color].
-    contradict owner_to_color.
-    firstorder using empty_in_iff.
-  Defined.
 
-  Local Lemma not_In_neq : forall (owner owner' : Owner.t) (coloring : Map.t nat), ~ Map.In owner coloring -> Map.In owner' coloring -> ~ Owner.eq owner owner'.
-  Proof.
-    intros owner owner' coloring not_In_owner In_owner'.
-    contradict not_In_owner.
-    now rewrite not_In_owner.
-  Defined.
-
-  Program Definition add_lt
-    (self : t | Ok self)
-    (owner : Owner.t | ~ Contains self owner)
-    (color : nat | color < colors self) :
-    {self' : t | Ok self'} :=
-    (colors self, Map.add owner (`color) (labeling self)).
-  Next Obligation.
-    rename H0 into not_In_owner, H into color_lt_colors, H1 into Ok_self.
-    intros n.
-    split.
-      intros n_lt_colors.
-      apply Ok_self in n_lt_colors as [owner' owner'_to_n].
-      exists owner'; apply Map.add_2 with (2 := owner'_to_n).
-      contradict not_In_owner.
-      unfold Contains.
-      rewrite not_In_owner; now exists n.
-    intros [owner' owner'_to_n].
-    apply add_mapsto_iff in owner'_to_n as [(_ & ->)| (_ & owner'_to_n)].
-      assumption.
-    now apply Ok_self; exists owner'.
-  Defined.
+  Definition add_lt
+    (self : t)
+    (owner : Owner.t)
+    (color : nat) :
+    t :=
+    (colors self, Map.add owner color (labeling self)).
 
   Program Definition add_eq
-    (self : t | Ok self)
-    (owner : Owner.t | ~ Contains self owner) :
-    {self' : t | Ok self'} :=
+    (self : t)
+    (owner : Owner.t) :
+    t :=
     (S (colors self), Map.add owner (colors self) (labeling self)).
-  Next Obligation.
-    rename H into not_In, H0 into Ok_self.
-    split.
-      intros color_lt_S_colors.
-      apply Lt.lt_n_Sm_le, PeanoNat.Nat.le_lteq in color_lt_S_colors as [color_lt_colors| ->].
-        apply Ok_self in color_lt_colors as [owner' owner'_to_color].
-        exists owner'.
-        apply Map.add_2.
-          apply not_In_neq with (Coloring.labeling self); firstorder.
+
+  Module Ok.
+    Definition t (coloring : Coloring.t) : Prop :=
+      forall color : nat,
+        color < colors coloring <->
+        (exists owner : Owner.t, MapsTo coloring owner color).
+
+    Lemma empty : t Coloring.empty.
+      intros color.
+      split.
+        intros color_lt_colors.
+        contradict color_lt_colors; auto with arith.
+      intros [owner owner_to_color].
+      contradict owner_to_color.
+      firstorder using empty_in_iff.
+    Qed.
+
+    Local Lemma not_In_neq : forall (owner owner' : Owner.t) (coloring : Map.t nat), ~ Map.In owner coloring -> Map.In owner' coloring -> ~ Owner.eq owner owner'.
+    Proof.
+      intros owner owner' coloring not_In_owner In_owner'.
+      contradict not_In_owner.
+      now rewrite not_In_owner.
+    Qed.
+
+    Lemma add_lt (self : Coloring.t) (owner : Owner.t) (color : nat) :
+      t self ->
+      ~ Coloring.Contains self owner ->
+      color < colors self ->
+      t (Coloring.add_lt self owner color).
+    Proof.
+      intros Ok_self not_In_owner color_lt_colors n.
+      split.
+        intros n_lt_colors.
+        apply Ok_self in n_lt_colors as [owner' owner'_to_n].
+        exists owner'; apply Map.add_2 with (2 := owner'_to_n).
+        contradict not_In_owner.
+        unfold Contains.
+        rewrite not_In_owner; now exists n.
+      intros [owner' owner'_to_n].
+      apply add_mapsto_iff in owner'_to_n as [(_ & ->)| (_ & owner'_to_n)].
         assumption.
-      now exists owner; apply Map.add_1.
-    intros [owner' owner'_to_color].
-    apply add_mapsto_iff in owner'_to_color as [[eq <-]| [neq owner'_to_color]].
-      auto.
-    apply PeanoNat.Nat.lt_lt_succ_r, Ok_self.
-    now exists owner'.
-  Defined.
+      now apply Ok_self; exists owner'.
+    Qed.
+
+    Lemma add_eq (self : Coloring.t) (owner : Owner.t) :
+      t self ->
+      ~ Coloring.Contains self owner ->
+      t (Coloring.add_eq self owner).
+    Proof.
+      intros Ok_self not_In_owner.
+      split.
+        intros color_lt_S_colors.
+        apply Lt.lt_n_Sm_le, PeanoNat.Nat.le_lteq in color_lt_S_colors as [color_lt_colors| ->].
+          apply Ok_self in color_lt_colors as [owner' owner'_to_color].
+          exists owner'.
+          apply Map.add_2.
+            apply not_In_neq with (Coloring.labeling self); firstorder.
+          assumption.
+        now exists owner; apply Map.add_1.
+      intros [owner' owner'_to_color].
+      apply add_mapsto_iff in owner'_to_color as [[eq <-]| [neq owner'_to_color]].
+        auto.
+      apply PeanoNat.Nat.lt_lt_succ_r, Ok_self.
+      now exists owner'.
+    Defined.
+  End Ok.
 End Coloring.
