Assigned.v
@@ -1,0 +1,719 @@
+Set Implicit Arguments.
+
+Require Import Coq.Structures.Equalities Coq.Structures.EqualitiesFacts.
+Require Import Coq.Lists.List Coq.Lists.SetoidList.
+
+Require Import Coq.Program.Program.
+
+Require Coq.FSets.FMaps.
+
+Import ListNotations.
+
+Require Import Shuffle.Instruction.
+Require Import Shuffle.Coloring.
+
+Module Opcode <: UsualDecidableType.
+  Inductive Opcode : Set :=
+  | Up : Opcode
+  | Down : Opcode.
+
+  Definition t : Type := Opcode.
+
+  Include HasUsualEq.
+  Include UsualIsEq.
+
+  Definition eq_dec : forall x y : t, {x = y} + {x <> y}.
+  Proof.
+    decide equality.
+  Qed.
+
+  Lemma not_Up_iff_Down : forall opcode : t, Up <> opcode <-> Down = opcode.
+  Proof.
+    now intros [|].
+  Defined.
+
+  Lemma not_Down_iff_Up : forall opcode : t, Down <> opcode <-> Up = opcode.
+  Proof.
+    now intros [|].
+  Defined.
+End Opcode.
+
+Section Option.
+  Variable (A B : Type).
+
+  Definition bind (mx : option A) (f : A -> option B) : option B :=
+    match mx with
+    | Some x => f x
+    | None => None
+    end.
+  Definition then' (mx : option A) (my : option B) : option B :=
+      bind mx (fun _ => my).
+  Definition ret (a : A) : option A :=
+    Some a.
+End Option.
+
+Module Assigned (Owner : DecidableType).
+  Module Instruction := Instruction Opcode Owner.
+
+  Lemma not_InA_cons : forall (A : Type) (eqA : A -> A -> Prop) (u v₀ : A) (y₀ : list A),
+    ~ InA eqA u (v₀ :: y₀) <->
+    ~ eqA u v₀ /\ ~ InA eqA u y₀.
+  Proof.
+    intros A eqA u v₀ y₀.
+    rewrite InA_cons; firstorder.
+  Qed.
+
+  Module Ok.
+    Notation add_Up owner instructions :=
+      ((Opcode.Up, owner) :: instructions).
+
+    Notation add_Down owner instructions :=
+      ((Opcode.Down, owner) :: instructions).
+
+    Definition InUp (owner : Owner.t) (instructions : list Instruction.t) : Prop :=
+      InA Instruction.eq (Opcode.Up, owner) instructions.
+
+    Definition InDown (owner : Owner.t) (instructions : list Instruction.t) : Prop :=
+      InA Instruction.eq (Opcode.Down, owner) instructions.
+
+    Ltac In_aux :=
+      unfold InUp, InDown; 
+      rewrite InA_cons;
+      firstorder using Opcode.not_Up_iff_Down.
+
+    Lemma InUp_add_Up
+      (owner owner' : Owner.t)
+      (instructions : list Instruction.t) :
+      InUp owner (add_Up owner' instructions) <->
+      Owner.eq owner owner' \/ InUp owner instructions.
+    Proof.
+      In_aux.
+    Qed.
+
+    Lemma InUp_add_Down
+      (owner owner' : Owner.t)
+      (instructions : list Instruction.t) :
+      InUp owner (add_Down owner' instructions) <->
+      InUp owner instructions.
+    Proof.
+      In_aux.
+    Qed.
+
+    Lemma InDown_add_Up
+      (owner owner' : Owner.t)
+      (instructions : list Instruction.t) :
+      InDown owner (add_Up owner' instructions) <->
+      InDown owner instructions.
+    Proof.
+      In_aux.
+    Qed.
+
+    Lemma InDown_add_Down
+      (owner owner' : Owner.t)
+      (instructions : list Instruction.t) :
+      InDown owner (add_Down owner' instructions) <->
+      Owner.eq owner owner' \/ InDown owner instructions.
+    Proof.
+      In_aux.
+    Qed.
+
+    Lemma not_InUp_add_Up
+      (owner owner' : Owner.t)
+      (instructions : list Instruction.t) :
+      ~ InUp owner (add_Up owner' instructions) <->
+      ~ Owner.eq owner owner' /\ ~ InUp owner instructions.
+    Proof.
+      firstorder using InUp_add_Up.
+    Qed.
+
+    Lemma not_InUp_add_Down
+      (owner owner' : Owner.t)
+      (instructions : list Instruction.t) :
+      ~ InUp owner (add_Down owner' instructions) <->
+      ~ InUp owner instructions.
+    Proof.
+      firstorder using InUp_add_Down.
+    Qed.
+
+    Lemma not_InDown_add_Up
+      (owner owner' : Owner.t)
+      (instructions : list Instruction.t) :
+      ~ InDown owner (add_Up owner' instructions) <->
+      ~ InDown owner instructions.
+    Proof.
+      firstorder using InDown_add_Up.
+    Qed.
+
+    Lemma not_InDown_add_Down
+      (owner owner' : Owner.t)
+      (instructions : list Instruction.t) :
+      ~ InDown owner (add_Down owner' instructions) <->
+      ~ Owner.eq owner owner' /\ ~ InDown owner instructions.
+    Proof.
+      firstorder using InDown_add_Down.
+    Qed.
+
+    Definition Active (owner : Owner.t) (instructions : list Instruction.t) : Prop :=
+      ~ InUp owner instructions /\
+      InDown owner instructions.
+
+    Inductive Ok : list Instruction.t -> Prop :=
+    | nil : Ok []
+    | cons_Up : forall (owner : Owner.t) (tail : list Instruction.t),
+      Ok tail ->
+      Active owner tail ->
+      Ok ((Opcode.Up, owner) :: tail)
+    | cons_Down : forall (owner : Owner.t) (tail : list Instruction.t),
+      Ok tail ->
+      ~ InDown owner tail -> 
+      Ok ((Opcode.Down, owner) :: tail).
+
+    Lemma cons_Up_iff : forall (owner : Owner.t) (tail : list Instruction.t), 
+      Ok ((Opcode.Up, owner) :: tail) <->
+        Active owner tail /\
+        Ok tail.
+    Proof.
+      intros.
+      now split; [inversion_clear 1| constructor].
+    Qed.
+
+    Lemma cons_Down_iff : forall (owner : Owner.t) (tail : list Instruction.t),
+      Ok ((Opcode.Down, owner) :: tail) <->
+        ~ InDown owner tail /\
+        Ok tail.
+    Proof.
+      intros.
+      split.
+        now inversion_clear 1.
+      now constructor.
+    Qed.
+
+    Lemma InUp_impl_InDown : forall (owner : Owner.t) (instructions : list Instruction.t),
+      Ok instructions ->
+      InUp owner instructions ->
+      InDown owner instructions.
+    Proof.
+      intros owner instructions Ok_instructions.
+      induction Ok_instructions as [| owner' tail Ok_tail IHtail [not_In_Up not_In_Down]| owner' tail Ok_tail IHtail not_In_Down]; intros In_Up.
+          now apply InA_nil in In_Up.
+        constructor 2.
+        apply InA_cons in In_Up as [[_ owner_eq_owner']| In_Up].
+          change (Owner.eq owner owner') in owner_eq_owner'.
+          now rewrite owner_eq_owner'.
+        now apply IHtail.
+      apply InA_cons in In_Up as [[Up_eq_Down _]| In_Up].
+        change (Opcode.Up = Opcode.Down) in Up_eq_Down.
+        discriminate Up_eq_Down.
+      constructor 2.
+      now apply IHtail.
+    Qed.
+
+    Lemma not_InDown_impl_not_InUp : forall (owner : Owner.t) (instructions : list Instruction.t),
+      Ok instructions ->
+      ~ InDown owner instructions ->
+      ~ InUp owner instructions.
+    Proof.
+      firstorder using InUp_impl_InDown.
+    Qed.
+
+    Lemma Active_nil (owner : Owner.t) : ~ Active owner [].
+    Proof.
+      intros [not_InUp_owner InDown_owner].
+      apply InA_nil with (1 := InDown_owner).
+    Qed.
+
+    Lemma Active_cons_Up (owner owner' : Owner.t) (instructions : list Instruction.t) :
+      Active owner ((Opcode.Up, owner') :: instructions) <->
+        ~ Owner.eq owner owner' /\ Active owner instructions.
+    Proof.
+      unfold Active, InUp, InDown.
+      rewrite not_InA_cons, InA_cons, Instruction.neq_eq_opcode by reflexivity; simpl.
+      firstorder.
+    Qed.
+
+    Lemma Active_cons_Down (owner owner' : Owner.t) (instructions : list Instruction.t) :
+      Ok ((Opcode.Down, owner') :: instructions) ->
+      Active owner ((Opcode.Down, owner') :: instructions) <->
+      Owner.eq owner owner' \/ Active owner instructions.
+    Proof.
+      intros Ok_instructions.
+      unfold Active, InUp, InDown.
+      rewrite not_InA_cons, InA_cons.
+      apply cons_Down_iff in Ok_instructions as [not_InDown_owner' Ok_instructions].
+      split.
+        intros ((_ & not_InUp_owner) & [(_ & owner_eq_owner')| InDown_owner]); [now left| right].
+        now split.
+      intros [owner_eq_owner'| (not_InDown_owner & InDown_owner)].
+        firstorder.
+          now apply Instruction.neq_opcode, Opcode.not_Up_iff_Down.
+        rewrite owner_eq_owner'.
+        now apply not_InDown_impl_not_InUp.
+      firstorder.
+      now apply Instruction.neq_opcode.
+    Qed.
+
+    Lemma InUp_Active (owner owner' : Owner.t) (instructions : list Instruction.t) :
+      Active owner instructions ->
+      InUp owner' instructions ->
+      ~ Owner.eq owner owner'. (* TODO *)
+    Proof.
+        intros (not_InUp_owner & _) InUp_owner' owner_eq_owner'.
+        unfold InUp in *. (* TODO *)
+        now rewrite <- owner_eq_owner' in InUp_owner'.
+    Qed.
+
+    Lemma not_InDown_Active (owner owner' : Owner.t) (instructions : list Instruction.t) :
+      Active owner instructions ->
+      ~ InDown owner' instructions ->
+      ~ Owner.eq owner owner'. (* TODO *)
+    Proof.
+        intros (not_InUp_owner & InDown_owner) not_InDown_owner' owner_eq_owner'.
+        unfold InDown in *. (* TODO *)
+        now rewrite <- owner_eq_owner' in not_InDown_owner'.
+    Qed.
+  End Ok.
+(* 
+  Definition Rel : relation Instruction.t :=
+    fun self other =>
+    Owner.eq (Instruction.operand self) (Instruction.operand other) ->
+      Instruction.opcode self = Opcode.Up /\
+      Instruction.opcode other = Opcode.Down.
+
+  Definition Ok : list Instruction.t -> Prop :=
+    fun instructions => 
+    ForallOrdPairs Rel instructions /\ (forall owner : Owner.t, InA Instruction.eq (Opcode.Up, owner) instructions -> InA Instruction.eq (Opcode.Down, owner) instructions).
+
+  Definition Forall_iff : forall (A : Type) (P : A -> Prop) (u₀ : A) (x₀ : list A), Forall P (u₀ :: x₀) <-> P u₀ /\ Forall P x₀.
+  Proof.
+    intros A P u₀ x₀.
+    split.
+      intros Forall_x.
+      constructor.
+        now apply Forall_inv with x₀.
+      now apply Forall_inv_tail with u₀.
+    intros [P_u₀ Forall_x₀].
+    now constructor.
+  Defined.
+
+  Definition Forall_InA : forall (A : Type) (eqA : A -> A -> Prop) (P : A -> Prop), Proper (eqA ==> iff) P -> forall (u : A) (y : list A), InA eqA u y -> Forall P y -> P u.
+  Proof.
+    intros A eqA P Proper_P u y.
+    induction 1 as [v₀ y₀ u_eq_v₀| v₀ y₀ In_y₀ IHy₀]; intros P_y.
+      rewrite u_eq_v₀.
+      now apply Forall_inv with y₀.
+    now apply IHy₀, Forall_inv_tail with v₀.
+  Qed.
+
+  Lemma not_InA_iff : forall (A : Type) (eqA : A -> A -> Prop) (u : A) (y : list A), ~ InA eqA u y <-> Forall (fun v => ~ eqA u v) y.
+  Proof.
+    intros A eqA u y.
+    now rewrite InA_altdef, <- Forall_Exists_neg.
+  Qed.
+
+  Instance Instruction_Rel_Proper : forall instruction : Instruction.t, Proper (Instruction.eq ==> iff) ( Rel instruction).
+  Proof.
+    intros [opcode₁ owner₁] [opcode₂ owner₂] [opcode₃ owner₃] [H₁ H₂].
+    simpl in *.
+    simpl in *.
+    unfold Rel.
+    compute in *.
+    now rewrite H₁, H₂.
+  Defined.
+
+  Hint Resolve InA_nil : test.
+  Hint Resolve <- InA_nil : test.
+  Hint Constructors ForallOrdPairs : test.
+
+  Definition OkOk : forall instructions : list Instruction.t, Ok instructions -> Ok instructions.
+  Proof.
+    intros x Ok_x.
+    split.
+      induction Ok_x as [| x₀ Ok_x₀ IHx₀ owner not_InUp_owner In_Down_owner| x₀ Ok_x₀ IHx₀ owner not_In_Down_owner].
+          constructor.
+        constructor 2 with (2 := IHx₀).
+        eapply Forall_impl, not_InA_iff with (1 := not_InUp_owner).
+        intros [opcode' owner'] neq owner_eq_owner'.
+        now eapply Instruction.ap_left', Opcode.not_Up in neq.
+      constructor 2 with (2 := IHx₀).
+      assert (not_In_owner : Forall (fun instruction => ~ Owner.eq owner (Instruction.operand instruction)) x₀).
+        assert (not_In_Up_owner : ~ InA Instruction.eq (Opcode.Up, owner) x₀).
+          contradict not_In_Down_owner; now apply Up_impl_Down.
+        eapply Forall_impl.
+        2: {
+          apply Forall_and; apply not_InA_iff.
+            exact not_In_Up_owner.
+          exact not_In_Down_owner.
+        }
+        intros [[|] owner']; firstorder.
+      now apply Forall_impl with (2 := not_In_owner).
+    intros owner.
+    now apply Up_impl_Down.
+  Qed. *)
+
+  Module Block.
+    Import Coq.FSets.FMaps.
+
+  Module Owner' :=  Backport_DT Owner.
+  Module Regular (Map : WSfun Owner').
+    Module Import Facts := WFacts_fun Owner' Map.
+
+    Module Coloring := Coloring Owner' Map.
+    Definition Ok := Ok.Ok.
+
+    Lemma not_InA_iff : forall (A : Type) (eqA : A -> A -> Prop) (u : A) (y : list A),
+      ~ InA eqA u y <->
+      Forall (fun v => ~ eqA u v) y.
+    Proof.
+      intros A eqA u y.
+      now rewrite InA_altdef, <- Forall_Exists_neg.
+    Qed.
+
+    Definition Forall_iff : forall (A : Type) (P : A -> Prop) (u₀ : A) (x₀ : list A), Forall P (u₀ :: x₀) <-> P u₀ /\ Forall P x₀.
+    Proof.
+      intros A P u₀ x₀.
+      split.
+        intros Forall_x.
+        constructor.
+          now apply Forall_inv with x₀.
+        now apply Forall_inv_tail with u₀.
+      intros [P_u₀ Forall_x₀].
+      now constructor.
+    Defined.
+
+      Definition Coloring_Ok (instructions : list Instruction.t) (coloring : Coloring.t) : Prop :=
+        Coloring.Ok coloring /\ (forall owner : Owner.t,
+        (Ok.Active owner instructions ->
+        Coloring.Contains coloring owner) /\
+        (Ok.InUp owner instructions ->
+        ~ Coloring.Contains coloring owner)).
+
+    Module Color.
+      Definition Ok
+        (instructions : list Instruction.t)
+        (coloring : Coloring.t)
+        (color : nat) :
+        Prop :=
+        exists owner : Owner.t,
+          Coloring.MapsTo coloring owner color /\
+          ~ Ok.InDown owner instructions.
+      
+      Lemma add_Up_eq
+        (coloring : Coloring.t)
+        (instructions : list Instruction.t)
+        (color : nat)
+        (owner : Owner.t) :
+        Ok instructions coloring color ->
+        ~ Coloring.Contains coloring owner ->
+        Ok (Ok.add_Up owner instructions) (Coloring.add_eq coloring owner) color.
+      Proof.
+        intros (owner' & owner'_to_color & not_InDown_owner') not_In_owner.
+        unfold Ok.
+        exists owner'; split.
+          apply Map.add_2.
+            contradict not_In_owner.
+            unfold Coloring.Contains.
+            rewrite not_In_owner; now exists color.
+          assumption.
+        now apply Ok.not_InDown_add_Up.
+      Qed.
+
+      Lemma Color_Ok_add_Up_lt
+        (coloring : Coloring.t)
+        (instructions : list Instruction.t)
+        (color color' : nat)
+        (owner : Owner.t) :
+        Ok instructions coloring color ->
+        ~ Coloring.Contains coloring owner ->
+        Ok (Ok.add_Up owner instructions) (Coloring.add_lt coloring owner color') color.
+      Proof.
+        intros (owner' & owner'_to_color & not_InDown_owner') not_In_owner.
+        unfold Ok.
+        exists owner'; split.
+          apply Map.add_2.
+            contradict not_In_owner.
+            unfold Coloring.Contains.
+            rewrite not_In_owner; now exists color.
+          assumption.
+        now apply Ok.not_InDown_add_Up.
+      Qed.
+    End Color.
+
+    Fixpoint regular
+      (instructions : list Instruction.t)
+      (coloring : Coloring.t)
+      (unused_colors : list nat) :
+      option Coloring.t :=
+      match instructions, unused_colors with
+      | (Opcode.Up, owner) :: tail, [] => regular
+        tail
+        (Coloring.add_eq coloring owner)
+        []
+      | (Opcode.Up, owner) :: tail, color :: unused_colors => regular
+        tail
+        (Coloring.add_lt coloring owner color)
+        unused_colors
+      | (Opcode.Down, owner) :: tail, unused_colors =>
+          bind (Coloring.find' coloring owner) (fun color => 
+          regular
+            tail
+            coloring
+            (color :: unused_colors))
+      | [], _ => ret coloring
+      end.
+
+    Module Type InvariantType.
+      Parameter P : list Instruction.t -> Coloring.t -> list nat -> option Coloring.t -> Prop.
+
+      Section Properties.
+        Variable owner : Owner.t.
+        Variable instructions : list Instruction.t.
+        Variable coloring : Coloring.t.
+        Variable color : nat.
+        Variable unused_colors : list nat.
+        Variable result : option Coloring.t.
+
+        Parameter P_nil :
+          P [] coloring unused_colors (Some coloring).
+
+        Parameter P_Up_eq :
+          P instructions (Coloring.add_eq coloring owner) [] result ->
+          P ((Opcode.Up, owner) :: instructions) coloring [] result.
+
+        Parameter P_Up_lt :
+          P instructions (Coloring.add_lt coloring owner color) unused_colors result ->
+          P ((Opcode.Up, owner) :: instructions) coloring (color :: unused_colors) result.
+
+        Parameter P_Down_Some :
+          Coloring.MapsTo coloring owner color ->
+          P instructions coloring (color :: unused_colors) result ->
+          P ((Opcode.Down, owner) :: instructions) coloring unused_colors result.
+
+        Parameter P_Down_None :
+          ~ Coloring.Contains coloring owner ->
+          P ((Opcode.Down, owner) :: instructions) coloring unused_colors None.
+      End Properties.
+    End InvariantType.
+
+    Module InvariantFacts (Import I : InvariantType).
+      Lemma correct : forall
+        (instructions : list Instruction.t)
+        (coloring : Coloring.t)
+        (unused_colors : list nat),
+        P instructions coloring unused_colors (regular instructions coloring unused_colors).
+      Proof.
+        induction instructions as [| [[|] owner] instructions IHinstructions];
+        intros
+          coloring
+          unused_colors.
+            apply P_nil.
+          destruct unused_colors as [| color unused_colors]; simpl.
+            specialize (IHinstructions (Coloring.add_eq coloring owner) []).
+            now apply P_Up_eq.
+          specialize (IHinstructions (Coloring.add_lt coloring owner color) unused_colors).
+          now apply P_Up_lt.
+        simpl.
+        destruct (Coloring.find' coloring owner) as [color|] eqn: find; simpl.
+          specialize (IHinstructions coloring (color :: unused_colors)).
+          apply find_mapsto_iff in find.
+          now apply P_Down_Some with color.
+        apply not_find_in_iff in find.
+        now apply P_Down_None.
+      Qed.
+    End InvariantFacts.
+
+    Definition UnusedColors_Ok
+      (coloring : Coloring.t)
+      (instructions : list Instruction.t)
+      (unused_colors : list nat) :
+      Prop :=
+      Forall (Color.Ok instructions coloring) unused_colors.
+
+    Inductive Subsets (A : Type) (P : list A -> Prop) : list A -> Prop :=
+    | Subsets_nil : Subsets P []
+    | Subsets_cons : forall (u₀ : A) (x₀ : list A),
+      P (u₀ :: x₀) -> Subsets P x₀ -> Subsets P (u₀ :: x₀).
+
+    Definition RealColoring
+      (coloring : Coloring.t)
+      (instructions : list Instruction.t) :
+      Prop :=
+      forall owner owner' : Owner.t,
+        ~ Owner.eq owner owner' ->
+        Ok.Active owner instructions ->
+        Ok.Active owner' instructions ->
+        exists color color' : nat,
+          Coloring.MapsTo coloring owner color /\
+          Coloring.MapsTo coloring owner' color' /\
+          color <> color'.
+
+    Inductive OptionSpec (A : Type) (P : A -> Prop) (Q : Prop) : option A -> Prop :=
+    | OptionSpec_Some : forall u : A, P u -> OptionSpec P Q (Some u)
+    | OptionSpec_None : Q -> OptionSpec P Q None.
+    #[global]
+    Hint Constructors OptionSpec : core.
+
+    Module Invariant <: InvariantType.
+      Definition P
+        (instructions : list Instruction.t)
+        (coloring : Coloring.t)
+        (unused_colors : list nat)
+        (result : option Coloring.t) :
+        Prop :=
+        Ok.Ok instructions ->
+        Coloring_Ok instructions coloring ->
+        UnusedColors_Ok coloring instructions unused_colors ->
+        OptionSpec Coloring.Ok False result.
+
+      Section Properties.
+        Variable owner : Owner.t.
+        Variable instructions : list Instruction.t.
+        Variable coloring : Coloring.t.
+        Variable color : nat.
+        Variable unused_colors : list nat.
+        Variable result : option Coloring.t.
+
+        Ltac P_intros :=
+          intros
+            Ok_instructions
+            [Ok_coloring Ok'_coloring]
+            Ok_unused_colors.
+
+        Lemma P_nil :
+          P [] coloring unused_colors (Some coloring).
+        Proof.
+          P_intros.
+          now constructor.
+        Qed.
+
+        Lemma P_Up_eq :
+          P instructions (Coloring.add_eq coloring owner) [] result ->
+          P ((Opcode.Up, owner) :: instructions) coloring [] result.
+        Proof.
+          intros IHP; P_intros.
+          apply Ok.cons_Up_iff in Ok_instructions as (Active_owner & Ok_instructions).
+          assert (not_In_owner : ~ Coloring.Contains coloring owner).
+            now apply Ok'_coloring; left.
+          apply IHP.
+              assumption.
+            split.
+              now apply Coloring.Ok.add_eq, Ok'_coloring; [| left].
+            intros owner'.
+            unfold Coloring.Contains; simpl.
+            rewrite add_in_iff.
+            split.
+              intros Active_owner'.
+              destruct (Owner.eq_dec owner owner') as
+                [owner_eq_owner'| owner_neq_owner'];
+                [now left| right].
+              apply Ok'_coloring, Ok.Active_cons_Up.
+              split.
+                now contradict owner_neq_owner'.
+              assumption.
+            intros InUp_owner'.
+            enough (~ Owner.eq owner owner' /\ ~ Map.In owner' (Coloring.labeling coloring)) by firstorder.
+            split.
+              now apply Ok.InUp_Active with instructions.
+            now apply Ok'_coloring; right.
+          constructor.
+        Qed.
+
+        Lemma P_Up_lt :
+          P instructions (Coloring.add_lt coloring owner color) unused_colors result ->
+          P ((Opcode.Up, owner) :: instructions) coloring (color :: unused_colors) result.
+        Proof.
+          intros IHP; P_intros.
+          apply Ok.cons_Up_iff in Ok_instructions as (Active_owner & Ok_instructions).
+          apply Forall_iff in Ok_unused_colors as (Ok_color & Ok_unused_colors).
+          assert (not_In_owner : ~ Coloring.Contains coloring owner).
+            now apply Ok'_coloring; left.
+          apply IHP.
+              assumption.
+            split.
+              apply Coloring.Ok.add_lt; try auto.
+              apply Ok_coloring.
+              destruct Ok_color as (owner' &  ? & ?).
+              now exists owner'.
+            intros owner'.
+            unfold Coloring.Contains; simpl.
+            rewrite add_in_iff.
+            split.
+            intros Active_owner'.
+            destruct (Owner.eq_dec owner owner') as
+              [owner_eq_owner'| owner_neq_owner'];
+              [now left| right].
+            apply Ok'_coloring, Ok.Active_cons_Up.
+              split.
+                now contradict owner_neq_owner'.
+              assumption.
+            intros InUp_owner'.
+            enough (~ Owner.eq owner owner' /\ ~ Map.In owner' (Coloring.labeling coloring)) by firstorder.
+            split.
+              now apply Ok.InUp_Active with instructions.
+            now apply Ok'_coloring; right.
+          eapply Forall_impl with (2 := Ok_unused_colors).
+          intros n (owner' & owner'_to_n & not_InDown_owner').
+          apply Ok.not_InDown_add_Up in not_InDown_owner'.
+          exists owner'; split; try assumption.
+          apply Map.add_2.
+            now apply Ok.not_InDown_Active with instructions.
+          assumption.
+        Qed.
+
+        Lemma P_Down_Some :
+          Coloring.MapsTo coloring owner color ->
+          P instructions coloring (color :: unused_colors) result ->
+          P ((Opcode.Down, owner) :: instructions) coloring unused_colors result.
+        Proof.
+          intros owner_to_color IHP; P_intros.
+          apply Ok.cons_Down_iff in Ok_instructions as (not_InUp_owner & Ok_tail).
+          unfold Coloring.find'.
+          apply IHP.
+              assumption.
+            split.
+              assumption.
+            intros owner'.
+            split.
+              intros Active_owner'.
+              now apply Ok'_coloring, Ok.Active_cons_Down; [constructor| right].
+            intros InUp_owner'.
+            now apply Ok'_coloring, Ok.InUp_add_Down.
+          constructor.
+          exists owner.
+            now split.
+          eapply Forall_impl with (2 := Ok_unused_colors).
+          intros n (owner' & owner'_to_color & not_InDown_owner').
+          exists owner'; split.
+            assumption.
+          now apply Ok.not_InDown_add_Down in not_InDown_owner'.
+        Qed.
+
+        Lemma P_Down_None :
+          ~ Coloring.Contains coloring owner ->
+          P ((Opcode.Down, owner) :: instructions) coloring unused_colors None.
+        Proof.
+          intros not_In_owner; P_intros.
+          apply Ok.cons_Down_iff in Ok_instructions as (not_InUp_owner & Ok_tail).
+          contradict not_In_owner.
+          now apply Ok'_coloring, Ok.Active_cons_Down; constructor.
+        Qed.
+      End Properties.
+    End Invariant.
+
+    Module Import InvariantFacts' := InvariantFacts Invariant.
+    Lemma regular_Ok : forall
+      (instructions : list Instruction.t )
+      (coloring : Coloring.t)
+      (unused_colors : list nat),
+      Ok.Ok instructions ->
+      Coloring_Ok instructions coloring ->
+      UnusedColors_Ok coloring instructions unused_colors ->
+      OptionSpec
+        (Coloring.Ok.t)
+        False
+        (regular instructions coloring unused_colors).
+    Proof.
+      apply correct.
+    Qed.
+  End Regular.
+End Block.
+End Assigned.
